Simulator/CoqSim/SimTypes.v
@@ -1,9 +1,9 @@
-Require Import String Fin.
+Require Import String Fin Kami.All.
 
-Class IsMap (M : Type -> Type -> Type) := {
-  empty : forall {K V}, M K V;
-  map_lookup : forall {K V}, K -> M K V -> option V;
-  insert : forall {K V}, K -> V -> M K V -> M K V
+Class StringMap (M : Type -> Type) := {
+  empty : forall {V}, M V;
+  map_lookup : forall {V}, string -> M V -> option V;
+  insert : forall {V}, string -> V -> M V -> M V
   }.
 
 Class IsVector (V : nat -> Type -> Type) := {
@@ -12,7 +12,8 @@ Class IsVector (V : nat -> Type -> Type) := {
   vec_eq : forall {X n}, (X -> X -> bool) -> V n X -> V n X -> bool;
   vec_to_list : forall {X n}, V n X -> list X;
   make_vec : forall {X n}, (Fin.t n -> X) -> V n X;
-  slice : forall {X n} (i m : nat), V n X -> (V m X)
+  slice : forall {X n} (i m : nat), V n X -> (V m X);
+  updates : forall {X n}, V n X -> list (nat * X) -> V n X
   }.
 
 Class IsWord (W : nat -> Type) := {
@@ -43,9 +44,13 @@ Class IsWord (W : nat -> Type) := {
 
   word_to_nat : forall {m}, W m -> nat;
   nat_to_word : forall {m}, nat -> W m;
+  
+  print_word_bin : forall {m}, W m -> string;
+  print_word_dec : forall {m}, W m -> string;
+  print_word_hex : forall {m}, W m -> string
   }.
 
-Class PrintMonad{W V}`{IsWord W, IsVector V} (M : Type -> Type) := {
+Class IOMonad{W V}`{IsWord W, IsVector V} (M : Type -> Type) := {
   ret : forall {X}, X -> M X;
   bind : forall {X Y}, M X -> (X -> M Y) -> M Y;
   error : forall {X}, string -> M X;
@@ -53,5 +58,7 @@ Class PrintMonad{W V}`{IsWord W, IsVector V} (M : Type -> Type) := {
   rand_bool : M bool;
   rand_word : forall n, M (W n);
   rand_vec : forall {X n}, M X -> M (V n X);
-  exit : forall {X}, M X
+  exit : forall {X}, M X;
   }.
+
+Notation "'io_do' x <- y ; cont" := (bind y (fun x => cont)) (at level 20).
