Simulator/CoqSim/Eval.v
@@ -1,5 +1,5 @@
-Require Import Compare_dec List String Streams.
-Import ListNotations.
+Require Import Compare_dec List String Streams FinFun.
+Import ListNotations Fin2Restrict.
 
 Require Import Kami.AllNotations.
 
@@ -16,7 +16,7 @@ Variable M : Type -> Type.
 
 Context `{IsWord Word}.
 Context `{IsVector Vec}.
-Context `{PrintMonad Word Vec M}.
+Context `{IOMonad Word Vec M}.
 
 Fixpoint eval_Kind(k : Kind) : Type :=
   match k with
@@ -26,19 +26,21 @@ Fixpoint eval_Kind(k : Kind) : Type :=
   | Array n k' => Vec n (eval_Kind k')
   end.
 
-Definition print_BF(bf : BitFormat) : nat -> string :=
+Definition print_BF(bf : BitFormat){n} : Word n -> string :=
   match bf with
-  | Binary => nat_binary_string
-  | Decimal => nat_decimal_string
-  | Hex => nat_hex_string
+  | Binary => print_word_bin
+  | Decimal => print_word_dec
+  | Hex => print_word_hex
   end.
+
+Axiom cheat : forall {X},X.
 
 Fixpoint print_Kind(k : Kind)(ff : FullFormat k) : eval_Kind k -> string :=
   match ff with
   | FBool n _ => fun x => space_pad n (if x then "1" else "0")
-  | FBit n m bf => fun x => zero_pad m (print_BF bf (word_to_nat x))
-  | FStruct n fk fs ffs => fun x => ("{" ++ String.concat "; " (v_to_list (vmap (fun '(str1,str2) => str1 ++ ":" ++ str2) (add_strings fs (tup_to_vec _ (fun i => print_Kind (ffs i)) x)))) ++ "}")%string
-  | FArray n k' ff' => fun _ => "arr" (*fix*)
+  | FBit n m bf => fun x => (*zero_pad m*) (print_BF bf x)
+  | FStruct n fk fs ffs => fun x => ("{ " ++ String.concat "; " (v_to_list (vmap (fun '(str1,str2) => str1 ++ ":" ++ str2) (add_strings fs (tup_to_vec _ (fun i => print_Kind (ffs i)) x)))) ++ "; }")%string
+  | FArray n k' ff' => fun x => ("[" ++ String.concat "; " (List.map (fun i => nat_decimal_string (f2n i) ++ "=" ++ print_Kind ff' (index i x)) (getFins n)) ++ "; ]")%string
   end.
 
 Fixpoint Kind_eq{k} : eval_Kind k -> eval_Kind k -> bool :=
@@ -56,6 +58,20 @@ Definition eval_FK(k : FullKind) :=
   end.
 
 Notation "'do' x <- y ; cont" := (bind y (fun x => cont)) (at level 20).
+
+Fixpoint default_val(k : Kind) : eval_Kind k :=
+  match k return eval_Kind k with
+  | Bool => false
+  | Bit n => nat_to_word 0
+  | Struct n ks fs => mkTup (fun i => eval_Kind (ks i)) (fun i => default_val (ks i))
+  | Array n k' => make_vec (fun _ => default_val k')
+  end.
+
+Definition default_val_FK(k : FullKind) : eval_FK k :=
+  match k with
+  | SyntaxKind k' => default_val k'
+  | NativeKind T t => t
+  end.
 
 Fixpoint rand_tuple{n} : forall ts : Fin.t n -> Type, (forall i, M (ts i)) -> M (Tuple ts) :=
   match n with
@@ -164,6 +180,9 @@ Fixpoint eval_Expr{k}(e : Expr eval_Kind k) : eval_FK k :=
   | BuildArray n k v => make_vec (fun i => eval_Expr (v i))
   end.
 
+Definition val_unpack(k : Kind) : Word (size k) -> eval_Kind k :=
+  fun w => eval_Expr (unpack _ (Const _ (ConstBit (natToWord _ (word_to_nat w))))).
+
 Definition eval_SysT(s : SysT eval_Kind) : M unit :=
   match s with
   | DispString s => print s
@@ -180,323 +199,5 @@ Fixpoint eval_list_SysT(xs : list (SysT eval_Kind)) : M unit :=
       )
   end.
 
-Section EvalAction.
-
-(* Variable KindInfo : Map string FullKind 
-Hypothesis ActionGood: forall Write r k in a, KindInfo r = k /\ forall Read r k in a, KindInfo r = k
-Lemma: SimRegGood: (r, k) in SimReg -> KindInfo r = k
-Theorem: ActionSimRegGood: forall Write r k in a, (r, k') in SimReg -> k = k' *)
-
-Definition SimReg := (string * {x : _ & fullType eval_Kind x})%type.
-Definition SimRegs := list SimReg.
-
-Variable regs : SimRegs.
-
-Record Update := {
-  reg_name : string;
-  kind : FullKind;
-  old_val : fullType eval_Kind kind;
-  new_val : fullType eval_Kind kind;
-  lookup_match : lookup String.eqb reg_name regs = Some (existT _ kind old_val)
-  }.
-
-Definition Updates := list Update.
-
-Fixpoint mkProd(ts : list Type) : Type :=
-  match ts with
-  | [] => unit
-  | T::ts' => (T * mkProd ts')%type
-  end.
-
-Fixpoint return_meth(meth : string)(sig : Signature)(meths : list (string * Signature)) : mkProd (List.map (fun dec => eval_Kind (fst (snd dec)) -> M (eval_Kind (snd (snd dec)))) meths) -> option (eval_Kind (fst (sig)) -> M (eval_Kind (snd (sig)))).
- refine match meths return mkProd (List.map (fun dec => eval_Kind (fst (snd dec)) -> M (eval_Kind (snd (snd dec)))) meths) -> option (eval_Kind (fst (sig)) -> M (eval_Kind (snd (sig)))) with
-  | [] => fun _ => None
-  | dec::meths' => match string_sigb (meth,sig) dec with
-                   | left pf => fun fs => Some _
-                   | right _ => fun fs => return_meth meth sig meths' (snd fs)
-                   end
-  end.
-Proof.
-  assert (sig = snd dec).
-  rewrite <- pf; auto.
-  rewrite H4.
-  exact (fst fs).
-Defined.
-
-Definition reg_not_found{X} : string -> M X :=
-  fun reg => error ("register " ++ reg ++ " not found.").
-
-Fixpoint wf_action{k}(a : ActionT eval_Kind k) : Prop :=
-  match a with
-  | MCall meth s e cont => forall x, wf_action (cont x)
-  | LetExpr k e cont => forall x, wf_action (cont x)
-  | LetAction k a cont => (wf_action a /\ forall x, wf_action (cont x))
-  | ReadNondet k cont => forall x, wf_action (cont x)
-  | ReadReg r k' cont => match lookup String.eqb r regs with
-                         | None => False
-                         | Some (existT k'' _) => k' = k'' /\ forall x, wf_action (cont x)
-                         end
-  | WriteReg r k' e a => match lookup String.eqb r regs with
-                         | None => False
-                         | Some (existT k'' _) => k' = k'' /\ wf_action a
-                         end
-  | IfElse e k1 a1 a2 cont => (wf_action a1 /\ wf_action a2 /\ forall x, wf_action (cont x))
-  | Sys _ a => wf_action a
-  | Return _ => True
-  end.
-
-Fixpoint eval_ActionT{k}(meths : list (string * Signature))(updates : Updates)(a : ActionT eval_Kind k)(a_wf : wf_action a)(fs : mkProd (List.map (fun dec => eval_Kind (fst (snd dec)) -> M (eval_Kind (snd (snd dec)))) meths)){struct a} : M (Updates * eval_Kind k).
-  refine (match a return wf_action a -> _ with
-  | MCall meth s e cont => fun pf => match return_meth meth s meths fs with
-                           | None => error ("Method " ++ meth ++ " not found")
-                           | Some f => (
-                                do v <- f (eval_Expr e);
-                                eval_ActionT _ meths updates (cont v) _ fs
-                                )
-                           end
-  | LetExpr k e cont => fun pf => eval_ActionT _ meths updates (cont (eval_Expr e)) _ fs
-  | LetAction k a cont => fun pf => (
-      do p <- eval_ActionT _ meths updates a _ fs;
-      eval_ActionT _ meths (fst p) (cont (snd p)) _ fs
-      )
-  | ReadNondet k cont => fun pf => (
-      do v <- rand_val_FK k;
-      eval_ActionT _ meths updates (cont v) _ fs
-      )
-  | ReadReg r k cont => fun pf=> match lookup String.eqb r regs with
-                        | None => reg_not_found r
-                        | Some p => _
-                        end
-  | WriteReg r k e a => fun pf => match lookup String.eqb r regs with
-                        | None => reg_not_found r
-                        | Some p => _
-                        end
-  | IfElse e k a1 a2 cont => fun pf => let a := if (eval_Expr e) then a1 else a2 in (
-      do p <- eval_ActionT _ meths updates a _ fs;
-      eval_ActionT _ meths (fst p) (cont (snd p)) _ fs
-      )
-  | Sys ss a => fun pf => (
-      do _ <- eval_list_SysT ss;
-      eval_ActionT _ meths updates a _ fs
-      )
-  | Return e => fun pf => ret (updates, eval_Expr e)
-  end a_wf).
-Proof.
-  - apply pf.
-  - apply pf.
-  - apply pf.
-  - apply pf.
-  - apply pf.
-  (* ReadReg *)
-  - destruct p.
-    simpl in pf.
-    destruct lookup in pf.
-    * destruct s; destruct pf as [keq pf'].
-      rewrite <- keq in f0.
-      exact (eval_ActionT _ meths updates (cont f0) (pf' _) fs).
-    * destruct pf.
-  (* WriteReg *)
-  - simpl in pf.
-    destruct lookup eqn:lk in pf.
-    * destruct s.
-      destruct pf as [keq pf'].
-      rewrite keq in e.
-      pose (upd := {|
-        reg_name := r;
-        kind := x;
-        old_val := f;
-        new_val := eval_Expr e;
-        lookup_match := lk
-        |}).
-      exact (eval_ActionT _ meths (upd::updates) a pf' fs).
-    * destruct pf.
-  - simpl in pf; destruct (eval_Expr e); tauto.
-  - apply pf.
-  - exact pf.
-Defined.
-
-Fixpoint curried(X : Type)(ts : list Type) : Type :=
-  match ts with
-  | [] => X
-  | T::ts' => T -> curried X ts'
-  end.
-
-Fixpoint curry(X : Type)(ts : list Type) : (mkProd ts -> X) -> curried X ts :=
-  match ts return (mkProd ts -> X) -> curried X ts with
-  | [] => fun f => f tt
-  | T::ts' => fun f t => curry ts' (fun xs => f (t,xs))
-  end.
-
-Definition eval_RuleT(meths : list (string * Signature))(r : RuleT)(r_wf : wf_action (snd r eval_Kind))(fs : mkProd (List.map (fun dec => eval_Kind (fst (snd dec)) -> M (eval_Kind (snd (snd dec)))) meths)) : M (Updates * eval_Kind Void) :=
-  eval_ActionT meths [] ((snd r) eval_Kind) r_wf fs.
-
-Fixpoint do_single_update(upd : Update)(regs : SimRegs) : SimRegs :=
-  match regs with
-  | [] => []
-  | (reg',v')::regs' => if String.eqb (reg_name upd) reg' then (reg', existT _ (kind upd) (new_val upd))::regs' else (reg',v')::do_single_update upd regs'
-  end.
-
-Definition do_updates(upds : Updates)(regs : SimRegs) : SimRegs :=
-  fold_right do_single_update regs upds.
-
-End EvalAction.
-
-Definition consistent(regs1 regs2 : SimRegs) := forall r k v,
-  lookup String.eqb r regs1 = Some (existT _ k v) -> exists v', lookup String.eqb r regs2 = Some (existT _ k v').
-
-Lemma consistent_refl : forall regs, consistent regs regs.
-Proof.
-  intros regs r k v lk.
-  exists v; auto.
-Qed.
-
-Lemma consistent_trans : forall regs1 regs2 regs3, consistent regs1 regs2 -> consistent regs2 regs3 -> consistent regs1 regs3.
-Proof.
-  intros regs1 regs2 regs3 cons12 cons23 r k v Hv.
-  destruct (cons12 r k v) as [v' Hv']; auto.
-  destruct (cons23 r k v') as [v'' Hv'']; auto.
-  exists v''; auto.
-Qed.
-
-Check lookup.
-
-Lemma lookup_cons : forall K V (eqb : K -> K -> bool) k k' v (ps : list (K*V)), lookup eqb k ((k',v)::ps) =
-  if eqb k k' then Some v else lookup eqb k ps.
-Proof.
-  intros.
-  unfold lookup.
-  unfold find.
-  simpl.
-  destruct (eqb k k'); auto.
-Qed.
-
-Lemma consistent_cons_cong : forall (regs1 regs2 : SimRegs)(r : SimReg), consistent regs1 regs2 -> consistent (r::regs1) (r::regs2).
-Proof.
-  intros regs1 regs2 r cons12 s k v Hv.
-  destruct r.
-  rewrite lookup_cons in Hv.
-  rewrite lookup_cons.
-  destruct (String.eqb s s0).
-  - exists v; auto.
-  - destruct (cons12 s k v); auto.
-    exists x; auto.
-Qed.
-
-(*
-Lemma consistent_do_update_cong : forall (regs1 regs2 : SimRegs)(upd : Update regs1),
-  consistent regs1 regs2 -> consistent (do_single_update upd regs1) (do_single_update upd regs2).
-Proof.
-Admitted.
-
-Lemma update_consistent : forall (regs : SimRegs)(upd : Update regs), consistent regs (do_single_update upd regs).
-Proof.
-  intros regs upd r k v Hv.
-  pose (lookup_match upd).
-  Print Update.
-*)
-
-Lemma wf_consistent_stable : forall {k} (a : ActionT eval_Kind k) regs1 regs2, consistent regs1 regs2 -> wf_action regs1 a -> wf_action regs2 a.
-Proof.
-  intros.
-  induction a; simpl.
-Admitted.
-
-Lemma updates_consistent : forall (regs : SimRegs)(upds : Updates regs), consistent regs (do_updates upds regs).
-Proof.
-  intros; induction upds; simpl.
-  - apply consistent_refl.
-  - apply (@consistent_trans _ (do_single_update a regs) _).
-Admitted.
-
-Lemma wf_updates_stable{k} : forall (regs : SimRegs)(upds : Updates regs)(a : ActionT eval_Kind k),
-  wf_action regs a -> wf_action (do_updates upds regs) a.
-Proof.
-  intros.
-  apply (@wf_consistent_stable _ _ regs).
-  - apply updates_consistent.
-  - auto.
-Qed.
-
-Definition maintain_wf{k} regs (upds : Updates regs) (a : ActionT eval_Kind k) : {r : RuleT & wf_action regs a} -> {r : RuleT & wf_action (do_updates upds regs) a}.
-Admitted.
-
-Fixpoint eval_Rules(timeout : nat)(meths : list (string * Signature))(init_regs : SimRegs)(rules : Stream {r : RuleT & wf_action init_regs (snd r eval_Kind)}){struct timeout} : mkProd (List.map (fun dec : string * (Kind * Kind) => eval_Kind (fst (snd dec)) -> M (eval_Kind (snd (snd dec)))) meths) -> M unit. refine
-  match timeout with
-  | 0 => fun fs => (
-      do _ <- print "TIMEOUT";
-      exit
-      )
-  | S timeout' => fun fs => match rules with
-                            | Cons r rules' => (
-                                do p <- eval_RuleT init_regs meths (projT1 r) (projT2 r)  fs;
-                                eval_Rules timeout' meths (do_updates (fst p) init_regs) (Streams.map _ rules') fs
-                                )
-                            end
-  end.
-Proof.
-  intros [rule wf].
-  exists rule.
-  apply wf_updates_stable; auto.
-Defined.
-
-Definition initialize_SimRegs(regs : list RegInitT) : SimRegs :=
-  List.map (fun '(r,existT k v) => match v return SimReg with
-                                   | None => (r,existT _ k (eval_ConstFullT (getDefaultConstFullKind k)))
-                                   | Some c => (r,existT _ k (eval_ConstFullT c))
-                                   end) regs.
-
-Lemma cons_neq{X}(x : X)(xs : list X) : x::xs <> [].
-Proof.
-  discriminate.
-Qed.
-
-Print RuleT.
-
-Fixpoint wf_rules(regs : SimRegs)(rules : list RuleT) :=
-  match rules with
-  | [] => True
-  | r::rs => wf_action regs (snd r eval_Kind) /\ wf_rules regs rs
-  end.
-
-Definition wf_bm(basemod : BaseModule) : Prop :=
-  match basemod with
-  | BaseRegFile rf => False
-  | BaseMod regs rules dms => wf_rules (initialize_SimRegs regs) rules
-  end.
-
-Definition get_wf_rules : forall regs rules, wf_rules (initialize_SimRegs regs) rules -> 
-  list {r : RuleT & wf_action (initialize_SimRegs regs) (snd r eval_Kind)}.
-Proof.
-  intros.
-  induction rules.
-  - exact [].
-  - simpl in H4; destruct H4.
-    exact ((existT _ a H4)::IHrules H5).
-Defined.
-
-Definition eval_Basemodule_rr(timeout : nat)(meths : list (string * Signature))(basemod : BaseModule)(wf : wf_bm basemod) : mkProd (List.map (fun dec : string * (Kind * Kind) => eval_Kind (fst (snd dec)) -> M (eval_Kind (snd (snd dec)))) meths) -> M unit. refine (
-  match basemod return wf_bm basemod -> _ with
-  | BaseRegFile rf => fun pf fs => _
-  | BaseMod regs rules dms =>
-      match rules with
-      | [] => fun _ _ => error "empty rules"
-      | r::rs => fun pf fs => _ (* eval_Rules timeout meths (initialize_SimRegs regs) (unwind_list (r::rs) (@cons_neq _ r rs)) *)
-      end
-  end wf).
-Proof.
-  - destruct pf.
-  - unfold wf_bm in pf.
-    refine (eval_Rules timeout meths (initialize_SimRegs regs) (unwind_list (get_wf_rules _ _ pf) _) fs).
-    simpl.
-    destruct pf; discriminate.
-Defined.
-
-Definition eval_BaseMod(timeout : nat)(meths : list (string * Signature))(basemod : BaseModule)(wf : wf_bm basemod) :=
-  curry _ (eval_Basemodule_rr timeout meths basemod wf).
-
 End Eval.
-
-Definition eval_BaseMod_Haskell := @eval_BaseMod HWord HVec IO _ _ _ _ _.
-
-Check eval_BaseMod_Haskell.
 
