Simulator/CoqSim/HaskellTypes.v
@@ -1,5 +1,6 @@
 Require Import Kami.Simulator.CoqSim.SimTypes.
 Require Extraction.
+Require Import String.
 
 Extraction Language Haskell.
 
@@ -7,22 +8,22 @@ Extraction Language Haskell.
 
 (* Maps *)
 
-Parameter HMap : Type -> Type -> Type.
+Parameter HMap : Type -> Type.
 
-Parameter Hempty : forall {K V}, HMap K V.
-Parameter Hmap_lookup : forall {K V}, K -> HMap K V -> option V.
-Parameter Hinsert : forall {K V}, K -> V -> HMap K V -> HMap K V.
+Parameter Hempty : forall {V}, HMap V.
+Parameter Hmap_lookup : forall {V}, string -> HMap V -> option V.
+Parameter Hinsert : forall {V}, string -> V -> HMap V -> HMap V.
 
-Instance HMapIsMap : IsMap HMap := {|
+Instance HMapIsMap : StringMap HMap := {|
   empty := @Hempty;
   map_lookup := @Hmap_lookup;
   insert := @Hinsert
   |}.
 
-Extract Constant HMap "k" "v" => "H.Map k v".
-Extract Constant Hempty => "H.empty".
-Extract Constant Hmap_lookup => "H.lookup".
-Extract Constant Hinsert => "H.insert".
+Extract Constant HMap "v" => "Data.Map.Map Prelude.String v".
+Extract Constant Hempty => "Data.Map.empty".
+Extract Constant Hmap_lookup => "Data.Map.lookup".
+Extract Constant Hinsert => "Data.Map.insert".
 
 (* Vectors *)
 
@@ -34,14 +35,16 @@ Parameter Heq : forall {X n}, (X -> X -> bool) -> HVec n X -> HVec n X -> bool.
 Parameter Hto_list : forall {X n}, HVec n X -> list X.
 Parameter Hmake_vec : forall {X n}, (Fin.t n -> X) -> HVec n X.
 Parameter Hslice : forall {X n} (i m : nat),  HVec n X -> HVec m X.
+Parameter Hupdates : forall {X n}, HVec n X -> list (nat * X) -> HVec n X.
 
 Instance HVecIsVec : IsVector HVec := {|
-  index := @Hindex;
+  SimTypes.index := @Hindex;
   vec_map := @Hmap;
   vec_eq := @Heq;
   vec_to_list := @Hto_list;
   make_vec := @Hmake_vec;
-  slice := @Hslice
+  slice := @Hslice;
+  updates := @Hupdates
   |}.
 
 Fixpoint Fin_to_list{X n} : (Fin.t n -> X) -> list X :=
@@ -57,6 +60,7 @@ Extract Constant Heq => "(\_ eqb v1 v2 -> Data.Vector.foldr (Prelude.&&) Prelude
 Extract Constant Hto_list => "(\ _ -> Data.Vector.toList)".
 Extract Constant Hmake_vec => "(\n f -> Data.Vector.fromList (coq_Fin_to_list n f))".
 Extract Constant Hslice => "(\_ i m v -> Data.Vector.slice i m v)".
+Extract Constant Hupdates => "(\_ -> (Data.Vector.//))".
 
 (* Words *)
 
@@ -83,6 +87,9 @@ Parameter Hwltb : forall {m}, HWord m -> HWord m -> bool.
 Parameter Hweqb : forall {m}, HWord m -> HWord m -> bool.
 Parameter Hword_to_nat : forall {m}, HWord m -> nat.
 Parameter Hnat_to_word : forall {m}, nat -> HWord m.
+Parameter Hprint_word_bin : forall {m}, HWord m -> string.
+Parameter Hprint_word_dec : forall {m}, HWord m -> string.
+Parameter Hprint_word_hex : forall {m}, HWord m -> string.
 
 Instance HWordIsWord : IsWord HWord := {|
   inv := @Hinv;
@@ -97,7 +104,7 @@ Instance HWordIsWord : IsWord HWord := {|
   sll := @Hsll;
   srl := @Hsrl;
   sra := @Hsra;
-  concat := @Hconcat;
+  SimTypes.concat := @Hconcat;
   add := @Hadd;
   mul := @Hmul;
   band := @Hband;
@@ -106,7 +113,10 @@ Instance HWordIsWord : IsWord HWord := {|
   wltb := @Hwltb;
   weqb := @Hweqb;
   word_to_nat := @Hword_to_nat;
-  nat_to_word := @Hnat_to_word
+  nat_to_word := @Hnat_to_word;
+  print_word_bin := @Hprint_word_bin;
+  print_word_dec := @Hprint_word_dec;
+  print_word_hex := @Hprint_word_hex
   |}.
 
 Extract Constant HWord => "Data.BitVector.BV".
@@ -131,7 +141,10 @@ Extract Constant Hbxor => "(\n -> Prelude.foldr Data.Bits.xor (Data.BitVector.ze
 Extract Constant Hwltb => "(\_ -> (Data.BitVector.<.))".
 Extract Constant Hweqb => "(\_ -> (Data.BitVector.==.))".
 Extract Constant Hword_to_nat => "(\_ x -> Prelude.fromIntegral (Data.BitVector.nat x))".
-Extract Constant Hnat_to_word => "Data.BitVector.bitVec".
+Extract Inlined Constant Hnat_to_word => "Data.BitVector.bitVec".
+Extract Constant Hprint_word_bin => "(\_ -> CustomExtract.bv_bin)".
+Extract Constant Hprint_word_dec => "(\_ -> CustomExtract.bv_dec)".
+Extract Constant Hprint_word_hex => "(\_ -> CustomExtract.bv_hex)".
 
 (* IO *)
 
@@ -147,7 +160,7 @@ Parameter Hrand_word : forall n, IO (HWord n).
 Parameter Hrand_vec : forall {X n}, IO X -> IO (HVec n X).
 Parameter Hexit : forall {X}, IO X.
 
-Instance IOPrintMonad : PrintMonad IO := {|
+Instance IOPrintMonad : IOMonad IO := {|
   ret := @Hret;
   bind := @Hbind;
   error := @Herror;
@@ -162,7 +175,8 @@ Extract Constant IO "a" => "Prelude.IO a".
 Extract Constant Hret => "Prelude.return".
 Extract Constant Hbind => "(GHC.Base.>>=)".
 Extract Constant Herror => "Prelude.error".
-Extract Constant Hprint => "Prelude.putStrLn".
+(*Extract Constant Hprint => "(\str -> (GHC.Base.>>) (Prelude.putStrLn str) (System.IO.hFlush System.IO.stdout))". *)
+Extract Constant Hprint => "Prelude.putStr".
 Extract Constant Hrand_bool => "Prelude.return Prelude.False". (*FIXME*)
 Extract Constant Hrand_word => "Prelude.undefined". (*FIXME*)
 Extract Constant Hrand_vec => "Prelude.undefined". (*FIXME*)
